Improved preprocessor constant folding, replaced computed min/max value operations by constants

thys/ds/LLVM_DS_Arith.thy
@@ -96,22 +96,189 @@ subsection \<open>Constant Folding\<close>
 (*
    TODO: No idea how complete these are 
 *)
-lemmas llvm_num_const_simps[llvm_inline] 
+lemmas llvm_num_const_simps[llvm_inline] =
+  arith_extra_simps
+  arith_simps arith_special 
+  more_arith_simps
+  nat_numeral_diff_1 diff_nat_numeral nat_numeral nat_0 nat_1 minus_nat.diff_0 
+  numeral_plus_one one_plus_numeral diff_minus_eq_add add_uminus_conv_diff
+  cancel_comm_monoid_add_class.diff_cancel 
+  pred_numeral_simps
+  Num.pow.simps power_numeral power_0 monoid_mult_class.power_one_right
+
+  word_of_int_numeral word_of_int_neg_numeral word_of_int_0 word_of_int_1  
+
+(* normalize word numerals to be positive and within range. *)    
+declaration \<open>fn _ => Named_Simpsets.map_ctxt @{named_simpset llvm_inline} (fn ctxt => 
+  ctxt addsimprocs [@{simproc unsigned_norm},@{simproc unsigned_norm_neg0},@{simproc unsigned_norm_neg1}])\<close>
+lemmas [llvm_inline] = minus_one_norm_num of_nat_numeral
+lemmas [llvm_inline] = len_of_numeral_defs  \<comment> \<open>Computation of LENGTH(_)\<close>
+  
+  
+  
+(* Regression test for constant folding *)  
+experiment
+begin                                                            
+
+  method ss = (simp named_ss llvm_inline: )
+
+  type_synonym w64 = "64 word"
+  type_synonym w1 = "1 word"
+  
+  (* nat + *)
+  schematic_goal "(3::nat) + 7 = numeral ?a" by ss
+  schematic_goal "(3::nat) + 0 = numeral ?a" by ss
+  schematic_goal "(3::nat) + 1 = numeral ?a" by ss
+  schematic_goal "(0::nat) + 7 = numeral ?a" by ss
+  schematic_goal "(1::nat) + 7 = numeral ?a" by ss
+  
+  (* int + *)
+  schematic_goal "(3::int) + 7 = numeral ?a" by ss
+  schematic_goal "(3::int) + 0 = numeral ?a" by ss
+  schematic_goal "(3::int) + 1 = numeral ?a" by ss
+  schematic_goal "(0::int) + 7 = numeral ?a" by ss
+  schematic_goal "(1::int) + 7 = numeral ?a" by ss
+  
+  schematic_goal "(3::int) + -7 = - numeral ?a" by ss
+  schematic_goal "(3::int) + -0 = numeral ?a" by ss
+  schematic_goal "(3::int) + -1 = numeral ?a" by ss
+  schematic_goal "(0::int) + -7 = - numeral ?a" by ss
+  schematic_goal "(1::int) + -7 = - numeral ?a" by ss
+
+  (* word 64 *)
+  schematic_goal "(3::w64) + 7 = numeral ?a" by ss
+  schematic_goal "(3::w64) + 0 = numeral ?a" by ss
+  schematic_goal "(3::w64) + 1 = numeral ?a" by ss
+  schematic_goal "(0::w64) + 7 = numeral ?a" by ss
+  schematic_goal "(1::w64) + 7 = numeral ?a" by ss
+  
+  schematic_goal "(-0::w64) = 0" by ss
+  schematic_goal "(-1::w64) = numeral ?a" by ss
+  schematic_goal "(-3::w64) = numeral ?a" by ss
+  
+  schematic_goal "(3::w64) + -0 = numeral ?a" by ss
+  schematic_goal "(3::w64) + -1 = numeral ?a" by ss
+  schematic_goal "(0::w64) + -7 = numeral ?a" by ss
+  schematic_goal "(1::w64) + -7 = numeral ?a" by ss
+  
+  schematic_goal "(3::w1) + 7 = 0" by ss
+  schematic_goal "(3::w1) + 0 = 1" by ss
+  schematic_goal "(3::w1) + 1 = 0" by ss
+  schematic_goal "(0::w1) + 7 = 1" by ss
+  schematic_goal "(1::w1) + 7 = 0" by ss
+  
+  schematic_goal "(-0::w1) = 0" by ss
+(*  schematic_goal "(-1::w1) = 1" by ss  
+  schematic_goal "(-3::w1) = 0" by ss TODO/FIXME: does not work yet*)
+  
+  schematic_goal "(3::w1) + -0 = 1" by ss
+  schematic_goal "(3::w1) + -1 = 0" by ss
+  (*
+  schematic_goal "(0::w1) + -7 = 1" by ss
+  schematic_goal "(1::w1) + -7 = numeral ?a" by ss TODO/FIXME: does not work yet*)
+  
+  (* nat - *)
+  schematic_goal "(9::nat) - 7 = numeral ?a" by ss
+  schematic_goal "(3::nat) - 0 = numeral ?a" by ss
+  schematic_goal "(3::nat) - 1 = numeral ?a" by ss
+  schematic_goal "(0::nat) - 0 = 0" by ss
+  schematic_goal "(1::nat) - 0 = 1" by ss
+  schematic_goal "(1::nat) - 1 = 0"  by ss
+  
+  (* int - *)
+  schematic_goal "(3::int) - 7 = -numeral ?a" by ss
+  schematic_goal "(3::int) - 0 = numeral ?a" by ss
+  schematic_goal "(3::int) - 1 = numeral ?a" by ss
+  schematic_goal "(0::int) - 7 = -numeral ?a" by ss
+  schematic_goal "(1::int) - 7 = -numeral ?a" by ss
+  schematic_goal "(0::int) - 0 = 0" by ss
+  schematic_goal "(1::int) - 0 = 1" by ss
+  schematic_goal "(1::int) - 1 = 0" by ss
+  
+  schematic_goal "(3::int) - -7 = numeral ?a" by ss
+  schematic_goal "(3::int) - -0 = numeral ?a" by ss
+  schematic_goal "(3::int) - -1 = numeral ?a" by ss
+  schematic_goal "(0::int) - -7 = numeral ?a" by ss
+  schematic_goal "(1::int) - -7 = numeral ?a" by ss
+  schematic_goal "(0::int) - -0 = 0" by ss
+  schematic_goal "(1::int) - -0 = 1" by ss
+  schematic_goal "(1::int) - -1 = numeral ?a" by ss
+
+  (* Powers (of 2) *)
+  schematic_goal "(2::nat)^0 = 1" by ss
+  schematic_goal "(2::nat)^1 = numeral ?a" by ss
+  schematic_goal "(2::nat)^3 = numeral ?a" by ss
+  schematic_goal "(2::nat)^4 = numeral ?a" by ss
+  schematic_goal "(2::nat)^5 = numeral ?a" by ss
+  schematic_goal "(2::nat)^6 = numeral ?a" by ss
+  schematic_goal "(2::nat)^7 = numeral ?a" by ss
+  schematic_goal "(2::nat)^8 = numeral ?a" by ss
+  schematic_goal "(2::nat)^16 = numeral ?a" by ss
+  schematic_goal "(2::nat)^32 = numeral ?a" by ss
+  schematic_goal "(2::nat)^64 = numeral ?a" by ss
+  schematic_goal "(2::nat)^128 = numeral ?a" by ss
+  
+  
+  schematic_goal "(2::int)^0 = 1" by ss
+  schematic_goal "(2::int)^1 = numeral ?a" by ss
+  schematic_goal "(2::int)^3 = numeral ?a" by ss
+  schematic_goal "(2::int)^4 = numeral ?a" by ss
+  schematic_goal "(2::int)^5 = numeral ?a" by ss
+  schematic_goal "(2::int)^6 = numeral ?a" by ss
+  schematic_goal "(2::int)^7 = numeral ?a" by ss
+  schematic_goal "(2::int)^8 = numeral ?a" by ss
+  schematic_goal "(2::int)^16 = numeral ?a" by ss
+  schematic_goal "(2::int)^32 = numeral ?a" by ss
+  schematic_goal "(2::int)^64 = numeral ?a" by ss
+  schematic_goal "(2::int)^128 = numeral ?a" by ss
+    
+
+end
+
+
+(* 
   = Num.arith_simps power_numeral pred_numeral_simps power_0
     arith_special numeral_One[symmetric]
-
+    len_of_numeral_defs word_of_int_numeral word_of_int_0 word_of_int_1 (* Computing LENGTH(numeral-type) *)
   
+    max_uint_def max_sint_def min_sint_def
+*)    
+    
 subsection \<open>Reflection of Maximum Representable Values\<close>  
   
-definition ll_max_uint :: "'l::len word llM" where [llvm_inline]: "ll_max_uint \<equiv> ll_sub 0 1"
-definition ll_max_sint :: "'l::len2 word llM" where [llvm_inline]: "ll_max_sint \<equiv> doM {r \<leftarrow> ll_max_uint; ll_lshr r 1}"
+lemmas [llvm_inline] = max_uint_def max_sint_def min_sint_def
+
+find_theorems "word_of_int (-_)"
+
+definition ll_max_uint :: "'l::len word llM" where [llvm_inline]: "ll_max_uint \<equiv> return (word_of_int (max_uint LENGTH('l) - 1))"
+definition ll_max_sint :: "'l::len2 word llM" where [llvm_inline]: "ll_max_sint \<equiv> return (word_of_int (max_sint LENGTH('l) - 1))"
+definition ll_min_sint :: "'l::len2 word llM" where [llvm_inline]: "ll_min_sint \<equiv> return (word_of_int (min_sint LENGTH('l) + 1))"
   
+(* TODO: Tuples will require some more thought. *)
+definition mk_pair :: "'a::llvm_rep \<Rightarrow> 'b::llvm_rep llM \<Rightarrow> ('a\<times>'b) llM" where
+  [llvm_inline]: "mk_pair a ctd \<equiv> doM { r\<leftarrow>ll_insert_fst init a; b\<leftarrow>ctd; ll_insert_snd r b }"
+
+experiment begin
+  (* Regression test to ensure that preprocessor does the computations. export-llvm will complain about non-numeral constants otherwise. *)
+  definition [llvm_code]: "test \<equiv> doM {
+    a\<leftarrow>(ll_max_uint :: 64 word llM);
+    b\<leftarrow>(ll_max_sint :: 64 word llM);
+    c\<leftarrow>(ll_min_sint :: 64 word llM);
+
+    d\<leftarrow>(ll_max_uint :: 1 word llM);
+    e\<leftarrow>(ll_max_sint :: 2 word llM);
+    f\<leftarrow>(ll_min_sint :: 2 word llM);
+      
+    mk_pair a (mk_pair b (mk_pair c (mk_pair d (mk_pair e (return f)))))
+  }"
+  
+  export_llvm "test"
+end
+
+
 context llvm_prim_arith_setup begin  
 
-lemma ll_max_uint_simp[vcg_normalize_simps]: "(ll_max_uint::'l::len word llM) = return (word_of_int (max_uint LENGTH('l) - 1))"
-  unfolding ll_max_uint_def max_uint_def
-  apply vcg_normalize
-  by (simp add: word_of_int_minus)
+lemmas [vcg_normalize_simps] = ll_max_uint_def ll_max_sint_def ll_min_sint_def
 
 lemma len_neq_one_conv: 
   "LENGTH('l::len) \<noteq> Suc 0 \<longleftrightarrow> (\<exists>n. LENGTH('l) = Suc (Suc n))"
@@ -133,7 +300,8 @@ proof -
   finally show ?thesis .
 qed  
  
-lemma ll_max_sint_simp[vcg_normalize_simps]: "(ll_max_sint::'l::len2 word llM) = return (word_of_int (max_sint LENGTH('l) - 1))"
+(*
+lemma ll_max_sint_simp[vcg_normalize_simps]: "(ll_max_sint::'l::len2 word llM) = consume1r ''sub'' (word_of_int (max_sint LENGTH('l) - 1))"
   unfolding ll_max_sint_def 
   supply [simp] = Suc_lessI max_sint_def max_uint_def len_neq_one_conv
   apply vcg_normalize
@@ -145,18 +313,19 @@ lemma ll_max_sint_simp[vcg_normalize_simps]: "(ll_max_sint::'l::len2 word llM) =
   apply (simp add: ll_max_sint_aux1)
   apply (smt one_le_power)
   by (simp add: pos_add_strict)
-    
+*)    
 
 lemma ll_max_uint_rule[vcg_rules]: "llvm_htriple \<box> (ll_max_uint::'l::len word llM) (\<lambda>r. \<up>(uint r = max_uint (LENGTH('l)) - 1))"
-  supply [simp] = max_uint_def zmod_minus1 uint_word_ariths
-  unfolding ll_max_uint_def max_uint_def
+  supply [simp] = max_uint_def zmod_minus1 uint_word_ariths word_of_int_inverse
   by vcg'
-    
-lemma ll_max_sint_rule: "llvm_htriple (\<box>) (ll_max_sint::'l::len2 word llM) (\<lambda>r. \<up>(uint r = max_sint LENGTH('l) - 1))"
-  apply vcg'
-  apply (auto simp add: uint_word_of_int max_sint_def)
-  by (smt diff_le_self int_mod_eq power_increasing_iff zless2p)
   
+lemma ll_max_sint_rule[vcg_rules]: "llvm_htriple (\<box>) (ll_max_sint::'l::len2 word llM) (\<lambda>r. \<up>(sint r = max_sint LENGTH('l) - 1))"
+  apply vcg'
+  by (simp add: max_sint_def sints_num word_sint.Abs_inverse)
+
+lemma ll_min_sint_rule[vcg_rules]: "llvm_htriple (\<box>) (ll_min_sint::'l::len2 word llM) (\<lambda>r. \<up>(sint r = min_sint LENGTH('l) + 1))"
+  apply vcg'
+  by (simp add: min_sint_def max_sint_def power_gt1_lemma word_sint.Abs_inverse)
 
 end  
   
